thys/Collections/ListSetImpl_Invar.thy
@@ -55,6 +55,7 @@ definition lsi_ball :: "'a lsi \<Rightarrow> ('a \<Rightarrow> bool) \<Rightarro
   where "lsi_ball l P == list_all P l"
 definition lsi_sel :: "'a lsi \<Rightarrow> ('a \<Rightarrow> 'r option) \<Rightarrow> 'r option" 
   where "lsi_sel == iti_sel lsi_iteratei"
+definition "lsi_sel' == SetGA.sel_sel' lsi_sel"
 
 definition lsi_to_list :: "'a lsi \<Rightarrow> 'a list" where "lsi_to_list == id"
 definition list_to_lsi :: "'a list \<Rightarrow> 'a lsi" where "list_to_lsi == remdups"
@@ -82,6 +83,7 @@ lemmas lsi_defs =
   lsi_inj_image_def
   lsi_ball_def
   lsi_sel_def
+  lsi_sel'_def
   lsi_to_list_def
   list_to_lsi_def
   lsi_size_def
@@ -132,6 +134,7 @@ lemma lsi_ball_impl: "set_ball lsi_\<alpha> lsi_invar lsi_ball"
 by(unfold_locales)(auto simp add: lsi_defs list_all_iff)
 
 lemmas lsi_sel_impl = iti_sel_correct[OF lsi_iteratei_impl, folded lsi_sel_def]
+lemmas lsi_sel'_impl = SetGA.sel_sel'_correct[OF lsi_sel_impl, folded lsi_sel'_def]
 
 lemma lsi_to_list_impl: "set_to_list lsi_\<alpha> lsi_invar lsi_to_list"
 by(unfold_locales)(auto simp add: lsi_defs)
@@ -159,6 +162,7 @@ interpretation lsi: set_image lsi_\<alpha> lsi_invar lsi_\<alpha> lsi_invar lsi_
 interpretation lsi: set_inj_image lsi_\<alpha> lsi_invar lsi_\<alpha> lsi_invar lsi_inj_image using lsi_inj_image_impl .
 interpretation lsi: set_ball lsi_\<alpha> lsi_invar lsi_ball using lsi_ball_impl .
 interpretation lsi: set_sel lsi_\<alpha> lsi_invar lsi_sel using lsi_sel_impl .
+interpretation lsi: set_sel' lsi_\<alpha> lsi_invar lsi_sel' using lsi_sel'_impl .
 interpretation lsi: set_to_list lsi_\<alpha> lsi_invar lsi_to_list using lsi_to_list_impl .
 interpretation lsi: list_to_set lsi_\<alpha> lsi_invar list_to_lsi using list_to_lsi_impl .
 interpretation lsi: set_size lsi_\<alpha> lsi_invar lsi_size using lsi_size_impl .
@@ -210,6 +214,7 @@ export_code
   lsi_inj_image
   lsi_ball
   lsi_sel
+  lsi_sel'
   lsi_to_list
   list_to_lsi
   lsi_size
